frontend/Frame.v
@@ -1,0 +1,46 @@
+(*
+ * Frame.v
+ * Wolf Honore
+ *
+ * Defines the abstract interface for stack frames.
+ *)
+
+Require Import String.
+
+Require Import Temp.
+Require Import Tree.
+
+Module Type FRAME.
+
+  Definition offset := nat.
+  Parameter frame : Set.
+
+  Parameter newFrame : nat -> list (frame * offset).
+  Parameter allocInFrame : frame -> offset.
+
+  Inductive frag : Set :=
+    | PROC : Temp.label -> Tree.stm -> frame -> frag
+    | DATA : Temp.label -> string -> frag.
+
+End FRAME.
+
+Module Frame <: FRAME.
+
+  Definition offset := nat.
+
+  Record frame' : Set := {
+    formals : nat;
+    offlst : list offset;
+    locals : nat;
+    maxargs : nat
+  }.
+  Definition frame := frame'.
+
+  Parameter newFrame : nat -> list (frame * offset).
+  Parameter allocInFrame : frame -> offset.
+
+  Inductive frag : Set :=
+    | PROC : Temp.label -> Tree.stm -> frame -> frag
+    | DATA : Temp.label -> string -> frag.
+
+End Frame.
