frontend/Temp.v
@@ -1,0 +1,37 @@
+(*
+ * Temp.v
+ * Wolf Honore
+ *
+ * Defines the type of temporary registers and label.
+ *)
+
+Require Import String.
+
+Require Import Symbol.
+Require Import Unique.
+
+Module Type TEMP (U : UNIQUE).
+
+  Definition temp := U.t.
+  Definition eq := U.eq.
+
+  Definition newTemp := U.new.
+
+  Definition label := Symbol.t.
+  Definition newLabel := SymUnique.new.
+  Parameter namedLabel : nat -> label.
+
+End TEMP.
+
+Module Temp <: TEMP NatUnique.
+
+  Definition temp := NatUnique.t.
+  Definition eq := NatUnique.eq.
+
+  Definition newTemp := NatUnique.new.
+
+  Definition label := Symbol.t.
+  Definition newLabel := SymUnique.new.
+  Definition namedLabel n := Symbol.symbol' n Symbol.sym_empty.
+
+End Temp.
