frontend/Translate.v
@@ -1,0 +1,59 @@
+(*
+ * Translate.v
+ * Wolf Honore
+ *
+ * Defines an interface for handling nested scope through
+ * static links.
+ *)
+
+Require Import Frame.
+Require Import Temp.
+Require Import Tree.
+Require Import Unique.
+
+Module Type TRANSLATE.
+
+  Parameter level : Set.
+  Parameter access : Set.
+  Parameter frag : Set.
+  Parameter gexp : Set.
+
+  Parameter outermost : level.
+  Parameter newLevel : forall A, level -> list A -> (level * list (A * access)).
+
+  Parameter allocInFrame : level -> access.
+  Parameter allocInRegister : access.
+
+  Parameter getResult : list frag.
+
+End TRANSLATE.
+
+Module Translate' (U : UNIQUE) <: TRANSLATE.
+
+  Inductive level' : Set :=
+    | TOP : level'
+    | LEVEL : Frame.frame -> nat -> level' -> U.t -> level'.
+  Definition level := level'.
+
+  Definition access := (level * nat)%type.
+
+  Definition frag := Frame.frag.
+
+  Inductive gexp' : Set :=
+    | Ex : Tree.exp -> gexp'
+    | Nx : Tree.stm -> gexp'
+    | Cx : Temp.label -> Temp.label -> Tree.stm -> gexp'.
+  Definition gexp := gexp'.
+
+  Definition outermost := TOP.
+  Definition newLevel {A} (par : level) (forms : list A) :=
+    (par, @nil (A * access)).
+
+  Definition allocInFrame (lvl : level) := (lvl, 0).
+  Definition allocInRegister := (outermost, 0).
+
+  Definition getResult := @nil frag.
+
+End Translate'.
+
+Module Translate := Translate' NatUnique.
