frontend/Tree.v
@@ -1,0 +1,137 @@
+(*
+ * Tree.v
+ * Wolf Honore
+ *
+ * Defines the intermediate representation of Tiger code in
+ * the form of a tree. The instructions are meant to be closer
+ * to assembly instructions.
+ *)
+
+Require Import QArith.
+
+Require Import Temp.
+
+Module Type TREE.
+
+  Parameter size : Set.
+
+  Inductive binop : Set :=
+    | FPLUS | FMINUS | FDIV | FMUL
+    | PLUS | MINUS | MUL | DIV
+    | AND | OR | LSHIFT | RSHIFT | ARSHIFT | XOR.
+
+  Inductive relop : Set :=
+    | EQ | NE | LT | GT | LE | GE
+    | ULT | ULE | UGT | UGE
+    | FEQ | FNE | FLT | FLE | FGT | FGE.
+
+  Inductive cvtop : Set :=
+    | CVTSU | CVTSS | CVTSF | CVTUU
+    | CVTUS | CVTFS | CVTFF.
+
+  Inductive stm : Set :=
+    | SEQ : stm -> stm -> stm
+    | LABEL : Temp.label -> stm
+    | JUMP : exp -> list Temp.label -> stm
+    | CJUMP : test -> Temp.label -> Temp.label -> stm
+    | MOVE : exp -> exp -> stm
+    | EXP : exp -> stm
+  with exp : Set :=
+    | BINOP : binop -> exp -> exp -> exp
+    | CVTOP : cvtop -> exp -> size -> size -> exp
+    | MEM : exp -> size -> exp
+    | TEMP : Temp.temp -> exp
+    | ESEQ : stm -> exp -> exp
+    | NAME : Temp.label -> exp
+    | CONST : nat -> exp
+    | CONSTF : Q -> exp
+    | CALL : exp -> list exp -> exp
+  with test : Set :=
+    | TEST : relop -> exp -> exp -> test.
+
+  Parameter notRel : relop -> relop.
+  Parameter commute : relop -> relop.
+
+End TREE.
+
+Module Tree <: TREE.
+
+  Definition label := Temp.label.
+  Definition temp := Temp.temp.
+  Definition size := nat.
+
+  Inductive binop : Set :=
+    | FPLUS | FMINUS | FDIV | FMUL
+    | PLUS | MINUS | MUL | DIV
+    | AND | OR | LSHIFT | RSHIFT | ARSHIFT | XOR.
+
+  Inductive relop : Set :=
+    | EQ | NE | LT | GT | LE | GE
+    | ULT | ULE | UGT | UGE
+    | FEQ | FNE | FLT | FLE | FGT | FGE.
+
+  Inductive cvtop : Set :=
+    | CVTSU | CVTSS | CVTSF | CVTUU
+    | CVTUS | CVTFS | CVTFF.
+
+  Inductive stm : Set :=
+    | SEQ : stm -> stm -> stm
+    | LABEL : Temp.label -> stm
+    | JUMP : exp -> list Temp.label -> stm
+    | CJUMP : test -> Temp.label -> Temp.label -> stm
+    | MOVE : exp -> exp -> stm
+    | EXP : exp -> stm
+  with exp : Set :=
+    | BINOP : binop -> exp -> exp -> exp
+    | CVTOP : cvtop -> exp -> size -> size -> exp
+    | MEM : exp -> size -> exp
+    | TEMP : Temp.temp -> exp
+    | ESEQ : stm -> exp -> exp
+    | NAME : Temp.label -> exp
+    | CONST : nat -> exp
+    | CONSTF : Q -> exp
+    | CALL : exp -> list exp -> exp
+  with test : Set :=
+    | TEST : relop -> exp -> exp -> test.
+
+  Definition notRel (f : relop) : relop :=
+    match f with
+    | EQ => NE
+    | NE => EQ
+    | LT => GE
+    | GE => LT
+    | GT => LE
+    | LE => GT
+    | ULT => UGE
+    | UGE => ULT
+    | ULE => UGT
+    | UGT => ULE
+    | FEQ => FNE
+    | FNE => FEQ
+    | FLT => FGE
+    | FGE => FLT
+    | FGT => FLE
+    | FLE => FGT
+    end.
+
+  Definition commute (f : relop) : relop :=
+    match f with
+    | EQ => EQ
+    | NE => NE
+    | LT => GT
+    | GE => LE
+    | GT => LT
+    | LE => GE
+    | ULT => UGT
+    | UGE => ULE
+    | ULE => UGE
+    | UGT => ULT
+    | FEQ => FEQ
+    | FNE => FNE
+    | FLT => FGT
+    | FGE => FLE
+    | FGT => FLT
+    | FLE => FGE
+    end.
+
+End Tree.
