util/Unique.v
@@ -1,0 +1,84 @@
+(*
+ * Unique.v
+ * Wolf Honore
+ *
+ * Defines an interface for a generator of unique values.
+ *)
+
+Require Import Le.
+Require Import List.
+Require Import Max.
+
+Module Type UNIQUE.
+
+  Parameter t : Set.
+
+  Parameter init : list t.
+  Parameter new : list t -> list t * t.
+  Parameter eq : forall (u1 u2 : t), {u1 = u2} + {u1 <> u2}.
+
+  Definition is_unique (us : list t) : Prop := NoDup us.
+
+  Hypothesis init_unique : is_unique init.
+
+  Hypothesis new_spec : forall u us us',
+    is_unique us ->
+    new us = (us', u) ->
+    In u us' /\ is_unique us'.
+
+End UNIQUE.
+
+Module NatUnique <: UNIQUE.
+
+  Definition t := nat.
+
+  Definition maximum (us : list t) := fold_right max 0 us.
+
+  Definition init := @nil t.
+
+  Definition new (us : list t) :=
+    let u := S (maximum us) in
+    (u :: us, u).
+
+  Definition eq : forall (u1 u2 : t), {u1 = u2} + {u1 <> u2}.
+    decide equality.
+  Defined.
+
+  Definition is_unique (us : list t) : Prop := NoDup us.
+
+  Lemma maximum_ge : forall u us,
+    In u us -> u <= maximum us.
+  Proof.
+    induction us; intros; inversion H; subst; simpl.
+    - destruct (max_dec u (maximum us)); rewrite e.
+      + constructor.
+      + rewrite <- e. apply le_max_l.
+    - apply IHus in H0.
+      destruct (max_dec a (maximum us)); rewrite e.
+      + assert (maximum us <= a).
+        { rewrite <- e. apply le_max_r. }
+        apply le_trans with (m := maximum us); assumption.
+      + assumption.
+  Qed.
+
+  Lemma init_unique : is_unique init.
+  Proof. constructor. Qed.
+
+  Lemma new_spec : forall u us us',
+    is_unique us ->
+    new us = (us', u) ->
+    In u us' /\ is_unique us'.
+  Proof.
+    unfold new, is_unique; intros.
+    inversion H0; subst.
+    split.
+    - simpl; left; reflexivity.
+    - destruct us.
+      + constructor; auto.
+      + constructor; [| assumption].
+        unfold not; intros.
+        apply maximum_ge in H1.
+        apply le_Sn_n in H1; assumption.
+  Qed.
+
+End NatUnique.
